examples/HolOmega/interim/dist_monadsScript.sml
@@ -8,8 +8,8 @@ struct
 open HolKernel Parse boolLib
      bossLib
 
-open categoryTheory KmonadTheory ;
-open auxLib ;
+open categoryTheory KmonadTheory GmonadTheory ;
+open auxLib ; infix RS RSN ;
 (*
 load "auxLib" ;
 load "dist_monadsTheory" ; open dist_monadsTheory ;
@@ -49,6 +49,72 @@ val Kcm_P3 = store_thm ("Kcm_P3",
    (FIRST_ASSUM (ASSUME_TAC o GSYM o MATCH_MP KmonDLU)),
    (ASM_REWRITE_TAC []) ]) ;
 
+val tm_Kcm_P14e = 
+  ``category (id, comp) /\ Kcmonad (id,comp) (unitM,extM,kcomp) /\
+    Kmonad [: ('A, 'M) Kleisli, 'N :] (unitM, kcomp) (unitNM, pext) /\
+    (extNM = (\:'a 'b. (\f. extM (pext [:'a, 'b:] f)))) ==>
+    (pext (comp (extNM f) g) = comp (extNM f) (pext g))`` ;
+
+val Kcm_P14e = store_thm ("Kcm_P14e", tm_Kcm_P14e,
+  EVERY [ STRIP_TAC,
+    (USE_LIM_RES_TAC (fn th => REWRITE_TAC [th]) Kc_cmD_pext),
+    TY_BETA_TAC, BETA_TAC,
+    (USE_LIM_RES_TAC ASSUME_TAC Kc_cmD_cm),
+    (farwmmp catDAss), (frrc_rewr KmonDAss) ]) ;
+
+(* note, to get Jones & Duponcheel P1 to P4,
+  have yet to show / assume (these are equivalent)
+  mapNM = mapM o mapN
+  pext (comp g f) = comp (pext g) (mapN f) 
+  kmap (comp g f) = comp (kmap g) (mapN f) 
+  *)
+  
+val Kdmonad_umj1' = TY_GEN_ALL (GEN_ALL Kdmonad_umj1) ;
+val Kdmonad_umj1'' = DISCH_ALL (TY_GEN_ALL (GEN_ALL (UNDISCH Kdmonad_umj1))) ;
+val Kdmonad_umj1_r = reo_prems rev Kdmonad_umj1 ;
+val Kdmonad_umj2_r = reo_prems rev Kdmonad_umj2 ;
+val Kdmonad_umj3_r = reo_prems rev Kdmonad_umj3 ;
+
+(* given monad N in the Kleisli category of monad M,
+  prove Jones & Duponcheel results about swap, where swap = kmap id,
+  and similar Barr & Wells results *)
+
+(* JD S3 is also BW D1 *)
+val tm_Kcm_S3 = 
+  ``category (id, comp) /\ Kmonad [:'A, 'M:] (id,comp) (unitM, extM) ==> 
+    Kdmonad [: ('A, 'M) Kleisli, 'N :] 
+      (unitM, Kcomp (id,comp) extM) (unitNM, pext, kmap, kjoin) ==>
+    (kmap (unitM [:'a:]) = unitM [:'a 'N:])`` ;
+
+val Kcm_S3 = store_thm ("Kcm_S3", tm_Kcm_S3,
+  EVERY [ (REPEAT STRIP_TAC),
+    (USE_LIM_RES_TAC ASSUME_TAC Kmonad_IMP_Kcat),
+    (*
+      (frrc_rewr Kdmonad_umj1') fails - BUG ?
+      (frrc_rewr Kdmonad_umj1) fails - BUG ?
+      also (frrc_rewr Kdmonad_umj1_r) works
+      *)
+    (frrc_rewr Kdmonad_umj1'') ]) ;
+
+(* before the last tactic, ie, before (frrc_rewr Kdmonad_umj1''), do:
+e (POP_ASSUM_LIST (MAP_EVERY ASSUME_TAC)) ;
+e (POP_ASSUM (fn _ => ALL_TAC)) ;
+val (sgs, goal) = top_goal () ;
+val [_, _, cat] = map ASSUME sgs ;
+val A = MATCH_MP Kdmonad_umj1'' cat ; 
+val B = MATCH_MP Kdmonad_umj1' cat ; 
+val C = MATCH_MP Kdmonad_umj1 cat ; 
+shouldn't B have two type quantifiers, as does A ?
+If removing the quantifiers is intended, still the types seem wrong,
+because in A there are distinct types 'M and 'N,
+which have become identified in A -
+see, eg, the type argument of Kdmonad,
+which is [:λα β. (α, β 'M) 'A, 'N:]in A,
+but is [:λα β. (α, β 'M) 'A, 'M:] in B
+Also look at C - similar to B ;
+note that TY_GEN_ALL (GEN_ALL C) has one type quantifier
+*)
+
 (*
 show_types := true ;
 show_types := false ;
@@ -56,6 +122,317 @@ handle e => Raise e ;
 set_goal ([], it) ;
 val (sgs, goal) = top_goal () ;
 *)
+
+(* JD S2 is also BW D2 *)
+val tm_Kcm_S2 = ``category (id, comp) /\
+    Kdmonad [:'A, 'M:] (id,comp) (unitM, extM, mapM, joinM) ==> 
+    Kdmonad [: ('A, 'M) Kleisli, 'N :] 
+      (unitM, Kcomp (id,comp) extM) (unitNM, pext, kmap, kjoin) ==>
+    (unitNM = \:'a. comp (unitM [:'a 'N:]) (unitN [:'a:])) ==> 
+    (comp (kmap (id [:'a 'M:])) (unitN [:'a 'M:]) = mapM unitN)`` ;
+
+val Kdmonad_IMP_Kcat = (KdmonadDK RSN (2, Kmonad_IMP_Kcat)) ;
+val Kcomp_thm' = SPEC_ALL (TY_SPEC_ALL (SPEC_ALL Kcomp_thm)) ;
+val Kcomp_thm'' = (TY_GEN_ALL (GEN_ALL Kcomp_thm')) ; 
+
+val Kcm_S2 = store_thm ("Kcm_S2", tm_Kcm_S2,
+  EVERY [ (REPEAT STRIP_TAC), (USE_LIM_RES_TAC ASSUME_TAC Kdmonad_IMP_Kcat),
+    (FIRST_REP_RES (MP_TAC o TY_GEN_ALL o REWRITE_RULE [Kcomp_thm'])
+      Kdmonad_umj3_r),
+    (ASM_REWRITE_TAC []), TY_BETA_TAC, (farwmmp catDAss),
+    (POP_ASSUM (fn _ => ALL_TAC)),
+    (POP_ASSUM (fn _ => ALL_TAC)),
+    (POP_ASSUM (fn _ => ALL_TAC)),
+    (FIRST_ASSUM (ASSUME_TAC o MATCH_MP KdmonadDK)),
+    (farwmmp KmonDRU), STRIP_TAC, (ASM_REWRITE_TAC []),
+    (USE_LIM_RES_TAC (fn th => REWRITE_TAC [th]) Kdmonad_extomap),
+    (farwmmp KmonDLU), (farwmmp catDLU), (farwmmp catDRU) ]) ; 
+
+val tm_Kcm_BWD3 = ``category (id, comp) /\
+    Kdmonad [:'A, 'M:] (id,comp) (unitM, extM, mapM, joinM) ==> 
+    Kdmonad [: ('A, 'M) Kleisli, 'N :] 
+      (unitM, Kcomp (id,comp) extM) (unitNM, pext, kmap, kjoin) ==>
+    (kmap joinM = comp (extM (kmap id)) (kmap id))`` ;
+
+val Kcm_BWD3 = store_thm ("Kcm_BWD3", tm_Kcm_BWD3,
+  EVERY [ (REPEAT STRIP_TAC), (USE_LIM_RES_TAC ASSUME_TAC Kdmonad_IMP_Kcat),
+    (FIRST_REP_RES (ASSUME_TAC o TY_GEN_ALL o 
+      GSYM o REWRITE_RULE [Kcomp_thm']) Kdmonad_umj2_r),
+    (ASM_REWRITE_TAC []), (farwmmp catDRU),
+    (frrc_rewr KdmonadD_JOINe) ]) ;
+
+(* with f = id, this is pext dorp = swap o_NM swap *)
+val tm_Kcm_S4_ss = ``category (id, comp) /\
+    Kmonad [:'A, 'M:] (id,comp) (unitM, extM) ==>
+    Kdmonad [: ('A, 'M) Kleisli, 'N :]
+      (unitM, Kcomp (id,comp) extM) (unitNM, pext, kmap, kjoin) ==>
+    (pext (extM (kmap f)) = comp (extM (pext (kmap f))) (kmap id))`` ;
+
+val Kcm_S4_ss = store_thm ("Kcm_S4_ss", tm_Kcm_S4_ss,
+  EVERY [ (REPEAT STRIP_TAC), (USE_LIM_RES_TAC ASSUME_TAC Kmonad_IMP_Kcat),
+   (USE_LIM_RES_TAC (fn th => REWRITE_TAC 
+     [REWRITE_RULE [Kcomp_thm'] (GSYM th)]) Kdmonad_extomap),
+   (farwmmp catDRU) ]) ;
+
+(* with f = g = id, this is swap o_NM swap = dorp o prod *)
+val tm_Kcm_S4_ss' = ``category (id, comp) /\
+    Kmonad [:'A, 'M:] (id,comp) (unitM, extM) ==>
+    Kdmonad [: ('A, 'M) Kleisli, 'N :]
+      (unitM, Kcomp (id,comp) extM) (unitNM, pext, kmap, kjoin) ==>
+    (comp (extM (pext (kmap f))) (kmap g) =
+      comp (extM (kmap f)) (pext g))`` ;
+
+val Kcm_S4_ss' = store_thm ("Kcm_S4_ss'", tm_Kcm_S4_ss',
+  EVERY [ (REPEAT STRIP_TAC), (USE_LIM_RES_TAC ASSUME_TAC Kmonad_IMP_Kcat),
+    (USE_LIM_RES_TAC (fn th => REWRITE_TAC [Kcomp_thm', th]) Kdmonad_umj4),
+    (farwmmp KmonDRAss), (farwmmp catDRAss),
+    AP_TERM_TAC, (farwmmp KdmonadD_JOIN_SYM), 
+    (USE_LIM_RES_TAC ((fn th => REWRITE_TAC [REWRITE_RULE [Kcomp_thm'] th]))
+      KdmonadD_EXT_SYM) ]) ;
+
+(* with g = id, this is swap o_M kjoin = kjoin o_M kmap swap *)
+val tm_Kcm_BWD4_alt = ``category (id, comp) /\
+    Kmonad [:'A, 'M:] (id,comp) (unitM, extM) ==> 
+    Kdmonad [: ('A, 'M) Kleisli, 'N :] 
+      (unitM, Kcomp (id,comp) extM) (unitNM, pext, kmap, kjoin) ==>
+    (comp (extM (kmap g)) kjoin = comp (extM kjoin) (kmap (kmap g)))`` ;
+
+val Kcm_BWD4_alt = store_thm ("Kcm_BWD4_alt", tm_Kcm_BWD4_alt,
+  EVERY [ (REPEAT STRIP_TAC), (USE_LIM_RES_TAC ASSUME_TAC Kmonad_IMP_Kcat),
+    (USE_LIM_RES_TAC ((fn th => REWRITE_TAC [th]) o
+      REWRITE_RULE [Kcomp_thm']) KdmonadD_EXT_SYM),
+    (frrc_rewr Kdmonad_umj4), (frrc_rewr KdmonadD_JOINe),
+    (REWRITE_TAC [Kcomp_thm]), (* fails - why ? - BUG ? *)
+    (REWRITE_TAC [Kcomp_thm']) (* succeeds *)
+    (* Note, (REWRITE_TAC [Kcomp_thm'']) also succeeds *)
+    ]) ;
+
+val tm_Kcm_S1 = ``category (id, comp) /\
+    Kdmonad [:'A, 'M:] (id,comp) (unitM, extM, mapM, joinM) ==> 
+    Kdmonad [: ('A, 'M) Kleisli, 'N :] 
+      (unitM, Kcomp (id,comp) extM) (unitNM, pext, kmap, kjoin) ==>
+    (extNM = (\:'a 'b. (\f. extM (pext [:'a, 'b:] f)))) ==>
+    (kmap (mapM f) = comp (extNM (comp unitNM f)) (kmap id))`` ;
+
+val Kcm_S1 = store_thm ("Kcm_S1", tm_Kcm_S1,
+  EVERY [ (REPEAT STRIP_TAC), (USE_LIM_RES_TAC ASSUME_TAC Kdmonad_IMP_Kcat),
+    (FIRST_REP_RES (fn th => ASM_REWRITE_TAC 
+      [MAPE_def, test_lhs_head_var "mapM" th]) KdmonadD_MAPe),
+    TY_BETA_TAC, BETA_TAC, 
+    (POP_ASSUM_LIST (MAP_EVERY ASSUME_TAC)),
+    (FIRST_ASSUM (fn th => 
+      (CONV_TAC o RATOR_CONV o RAND_CONV o RAND_CONV o REWR_CONV) 
+      (MATCH_MP (GSYM catDRU) th))),
+    (FIRST_REP_RES (fn th => CHANGED_TAC 
+      (REWRITE_TAC [REWRITE_RULE [Kcomp_thm'] th])) Kdmonad_umj2_r),
+    AP_THM_TAC, AP_TERM_TAC, AP_TERM_TAC,
+    (farwmmp KdmonadD_MAPe), (REWRITE_TAC [Kcomp_thm']), 
+    (farwmmp catDAss), (farwmmp (KdmonadDK RS KmonDRU)) ]) ;
+
+val Kdc_mon = (KdcmonadDK RS KdmonadDK) ;
+val KdcmonDRU = (Kdc_mon RS KmonDRU) ;
+  
+(* showing how JD S1 to S4 give the BW D1 to D4 and swap is nt ;
+  have that S2 is BWD2, S3 is BWD1, S1 is swap is nt ;
+  need to show 
+*)
+
+(*
+show_types := true ;
+show_types := false ;
+handle e => Raise e ;
+set_goal ([], it) ;
+val (sgs, goal) = top_goal () ;
+*)
+
+(* conditions S1 to S4 for monads, as in Jones & Duponcheel *)
+
+val S1to4_def = Define `S1to4 = 
+    (\: 'A 'N 'M. \ ((id, comp) : 'A category)
+    ((unitM, extM, mapM, joinM) : ('A, 'M) Kdmonad)
+    ((unitN, mapN, joinN) : ('A, 'N) g_umj_monad)
+    (swap : (! 'a. ('a 'M 'N, 'a 'N 'M) 'A)).
+    
+    (* S1 ; swap nt *) (!: 'a 'b. ! (f : ('a, 'b) 'A).
+      comp ((swap : (! 'a. ('a 'M 'N, 'a 'N 'M) 'A)) [:'b:]) (mapN (mapM f)) =
+      comp (mapM (mapN f)) (swap [:'a:])) /\
+    (* S2 ; BWD2 *) (!: 'a. comp (swap [:'a:]) unitN = mapM unitN) /\
+    (* S3 ; BWD1 *) (!: 'a. comp (swap [:'a:]) (mapN unitM) = unitM) /\
+    (* S4 *) (let (prod : (! 'a. ('a 'N 'M 'N, 'a 'N 'M) 'A)) =
+        \:'a. comp (mapM (joinN [:'a:])) (swap [:'a 'N:]) in
+      (!: 'a. comp (prod [:'a:]) (mapN (extM (swap [:'a:]))) = 
+        comp (extM (swap [:'a:])) (prod [:'a 'M:]))))` ;
+
+val S1to4_thm = save_thm ("S1to4_thm",
+  SPEC_ALL (TY_SPEC_ALL (mk_exp_thm'' S1to4_def))) ; 
+val (S1to4D, S1to4I) = EQ_IMP_RULE S1to4_thm ;
+val [S_1, S_2, S_3, S_4] = map DISCH_ALL (CONJUNCTS (UNDISCH S1to4D)) ;
+val _ = ListPair.map save_thm (["S_1","S_2","S_3","S_4"], [S_1,S_2,S_3,S_4]) ;
+
+(* distributive law for monads, as in Barr & Wells *)
+
+val dist_law_def = Define `dist_law = 
+    (\: 'A 'N 'M. \ ((id, comp) : 'A category)
+    ((unitM, extM, mapM, joinM) : ('A, 'M) Kdmonad)
+    ((unitN, mapN, joinN) : ('A, 'N) g_umj_monad)
+    (swap : (! 'a. ('a 'M 'N, 'a 'N 'M) 'A)).
+    (* S1 ; swap nt *) (!: 'a 'b. ! (f : ('a, 'b) 'A).
+      comp ((swap : (! 'a. ('a 'M 'N, 'a 'N 'M) 'A)) [:'b:]) (mapN (mapM f)) =
+      comp (mapM (mapN f)) (swap [:'a:])) /\
+    (* S2 ; BWD2 *) (!: 'a. comp (swap [:'a:]) unitN = mapM unitN) /\
+    (* S3 ; BWD1 *) (!: 'a. comp (swap [:'a:]) (mapN unitM) = unitM) /\
+    (* BWD3 *) (!: 'a. comp (swap [:'a:]) (mapN joinM) =
+      comp (extM (swap [:'a:])) (swap [:'a 'M:])) /\
+    (* BWD4 *) (!: 'a. comp (swap [:'a:]) joinN = 
+      comp (mapM joinN) (comp (swap [:'a 'N:]) (mapN (swap [:'a:])))))` ;
+
+val dist_law_thm = save_thm ("dist_law_thm",
+  SPEC_ALL (TY_SPEC_ALL (mk_exp_thm'' dist_law_def))) ; 
+val (dist_lawD, dist_lawI) = EQ_IMP_RULE dist_law_thm ;
+val [dlDnt, dlD1, dlD2, dlD3, dlD4] = 
+  map DISCH_ALL (CONJUNCTS (UNDISCH dist_lawD)) ;
+val _ = ListPair.map save_thm (["dlDnt", "dlD1", "dlD2", "dlD3", "dlD4"],
+  [dlDnt, dlD1, dlD2, dlD3, dlD4]) ;
+
+(* converse - assume swap is nt, and BW D1 to D4, show how to 
+  define a compound monad satisfying J1 and J2 *)
+val tmBWD_cm' = ``category (id, comp) ==>
+    Kdcmonad [:'A, 'M:] (id,comp) (unitM, extM, kcomp, mapM, joinM) ==> 
+    g_umj_monad [:'A, 'N:] (id,comp) (unitN, mapN, joinN) ==> 
+    dist_law (id,comp) (unitM,extM,mapM,joinM) (unitN,mapN,joinN) swap ==>
+    (kjoin = \:'a. comp unitM (joinN [:'a:])) ==>
+    (kmap = \:'a 'b. \f. comp swap (mapN [:'a, 'b 'M:] f)) ==>
+    (unitNM = \:'a. comp (unitM [:'a 'N:]) (unitN [:'a:])) ==>
+    (pext = \:'a 'b. \f. kcomp kjoin (kmap [:'a, 'b 'N:] f)) ==>
+  g_umj_monad [:('A,'M) Kleisli, 'N:] (unitM, kcomp) (unitNM, kmap, kjoin) ==>
+  S1to4 (id,comp) (unitM,extM,mapM,joinM) (unitN,mapN,joinN) swap ==> 
+  Kdmonad [:('A,'M) Kleisli, 'N:] (unitM,kcomp) (unitNM,pext,kmap,kjoin) ==>
+    (* S4 o extra *) (let (prod : (! 'a. ('a 'N 'M 'N, 'a 'N 'M) 'A)) =
+        \:'a. comp (mapM (joinN [:'a:])) (swap [:'a 'N:]) in
+      (!: 'a. comp (comp (prod [:'a:]) (mapN (extM (swap [:'a:])))) 
+	  (mapN (unitM [:'a 'M 'N:])) = 
+        comp (comp (extM (swap [:'a:])) (prod [:'a 'M:]))
+	  (mapN (unitM [:'a 'M 'N:]))) /\
+      (!: 'a. comp (comp (prod [:'a:]) (mapN (extM (swap [:'a:])))) 
+	  (mapN (mapM (unitN [:'a 'M:]))) = 
+        comp (comp (extM (swap [:'a:])) (prod [:'a 'M:]))
+	  (mapN (mapM (unitN [:'a 'M:])))) )`` ;
+  
+val ([cic, KmonM, umjN, dl, kjoin, kmap, unitNM, pext, umjK, S14, KdK], S4os) = 
+  strip_imp tmBWD_cm' ;
+
+(* TODO - prove S1to4 implies dist_law *)
+val tm_S_DL = list_mk_imp ([cic, KmonM, umjN, S14], dl) ;
+(*
+show_types := true ;
+show_types := false ;
+handle e => Raise e ;
+set_goal ([], it) ;
+val (sgs, goal) = top_goal () ;
+*)
+
+val S_DL = store_thm ("S_DL", tm_S_DL,
+  EVERY [ (REWRITE_TAC [S1to4_thm, dist_law_thm, LET_THM]),
+    BETA_TAC, TY_BETA_TAC, (STRIP_TAC), (STRIP_TAC), 
+    (STRIP_TAC), (STRIP_TAC), (SUBGOAL_THEN S4os MP_TAC) ]
+
+  THENL [
+    EVERY [ (REWRITE_TAC [LET_THM]),
+      BETA_TAC, TY_BETA_TAC, (ASM_REWRITE_TAC []) ],
+
+    EVERY [ (POP_ASSUM (fn _ => ALL_TAC)),
+      (ASM_REWRITE_TAC [LET_THM]), BETA_TAC, TY_BETA_TAC,
+
+      (* first one ie BWD4 *)
+      (farwmmp catDRAss), (farwmmp (GSYM g_umjD2)),
+      (farwmmp KdcmonDRU), (ASM_REWRITE_TAC []),
+      (FIRST_ASSUM (ASSUME_TAC o MATCH_MP KdcmonadDK)),
+      (frrc_rewr Kdmonad_umj3_r), (farwmmp catDAss), (farwmmp KdcmonDRU),
+      (* second one ie BWD3, some already done *)
+      (FIRST_ASSUM (CONV_TAC o CHANGED_CONV o
+	DEPTH_CONV o REWR_CONV o MATCH_MP catDRAss)),
+      (frrc_rewr (GSYM Kdmonad_umj2_r)), (farwmmp g_umjD6),
+      (frrc_rewr Kdmonad_umj1_r), (farwmmp catDLU),
+      (frrc_rewr (GSYM Kdmonad_extomap)), (ASM_REWRITE_TAC []),
+      (frrc_rewr Kdmonad_umj4), (farwmmp g_umjD2),
+      (FIRST_ASSUM (CONV_TAC o CHANGED_CONV o
+	DEPTH_CONV o REWR_CONV o MATCH_MP catDAss)),
+      (ASM_REWRITE_TAC []), (farwmmp catDAss),
+      (frrc_rewr (GSYM Kdmonad_umj2_r)), (farwmmp g_umjD6),
+      (frrc_rewr Kdmonad_umj1_r), (farwmmp catDLU),
+      (farwmmp KdmonadD_JOINe), (SRW_TAC [] []) ] ]) ;
+
+val tmBWD_cm = list_mk_imp ([cic, KmonM, umjN, dl, kjoin, kmap, unitNM], umjK);
+val tmBWD_cmK = list_mk_imp ([cic, KmonM, umjN, dl, kjoin, kmap, unitNM, pext],
+  KdK);
+
+(* note also, extM kjoin = mapM joinN, ie, J2 holds,
+   def'n of pext, and Kdmonad result omitted above is 
+    (pext = \:'a 'b. \f. kcomp kjoin (kmap [:'a, 'b 'N:] f)) ==>
+  Kdmonad [:('A,'M) Kleisli, 'N:] (unitM, kcomp) (unitNM, pext, kmap, kjoin)`` ;
+*)
+
+val ktacs2 = [ (FIRST_ASSUM (fn th => REWRITE_TAC [Kcomp_thm',
+    MATCH_MP KdcmonadD_Kcomp th])),
+  (USE_LIM_RES_TAC (fn th => REWRITE_TAC [th]) KdmonadD_EXTe),
+  (farwmmp g_umjD2), (farwmmp catDAss), (farwmmp dlD3),
+  (REPEAT STRIP_TAC), AP_THM_TAC, AP_TERM_TAC,
+  (farwmmp catDRAss), (farwmmp dlDnt), (farwmmp catDAss),
+  AP_THM_TAC, AP_TERM_TAC,
+  (USE_LIM_RES_TAC (fn th => REWRITE_TAC [th]) Kdmonad_umj2),
+  (USE_LIM_RES_TAC (fn th => REWRITE_TAC [th]) KdmonadD_EXTe),
+  (farwmmp catDAss)] ;
+
+val ktacs3 = [ (FIRST_ASSUM (fn th => REWRITE_TAC [Kcomp_thm',
+    MATCH_MP KdcmonadD_Kcomp th])),
+  (farwmmp catDAss), (farwmmp KdcmonDRU), 
+  (farwmmp catDRAss), (farwmmp g_umjD3),
+  (farwmmp catDAss), (farwmmp dlD1), (farwmmp KdmonadD_MAPe)] ;
+
+val ktacs4 = [ (FIRST_ASSUM (fn th => REWRITE_TAC [Kcomp_thm',
+    MATCH_MP KdcmonadD_Kcomp th])),
+  (farwmmp catDAss), (farwmmp KdcmonDRU),
+  (farwmmp catDRAss), (farwmmp g_umjD4),
+  (farwmmp catDAss), (farwmmp dlD4),
+  (farwmmp g_umjD2), (farwmmp catDAss), (farwmmp KdmonadD_MAPe)] ;
+
+val ktacs5 = [ (FIRST_ASSUM (fn th => REWRITE_TAC [Kcomp_thm',
+    MATCH_MP KdcmonadD_Kcomp th])),
+  (farwmmp catDAss), (farwmmp KdcmonDRU),
+  (farwmmp catDRAss), (farwmmp g_umjD5), (farwmmp catDRU)] ;
+
+val ktacs6 = [ (farwmmp g_umjD2), (farwmmp catDAss), (farwmmp dlD2),
+  (FIRST_ASSUM (fn th => REWRITE_TAC [Kcomp_thm',
+    MATCH_MP KdcmonadD_Kcomp th])),
+  (farwmmp catDAss), (farwmmp KdcmonDRU),
+  (farwmmp catDRAss), (farwmmp g_umjD6), (farwmmp catDRU)] ;
+
+val ktacs7 = [ (farwmmp g_umjD2), (farwmmp catDAss), (farwmmp dlD2),
+  (FIRST_ASSUM (fn th => REWRITE_TAC [Kcomp_thm',
+    MATCH_MP KdcmonadD_Kcomp th])),
+  (farwmmp catDAss), (farwmmp KdcmonDRU),
+  (farwmmp catDRAss), (farwmmp g_umjD7)] ;
+
+val BWD_cm = store_thm ("BWD_cm", tmBWD_cm, 
+  EVERY [ REPEAT STRIP_TAC,
+    (POP_ASSUM_LIST (MAP_EVERY (ASSUME_TAC o fix_abs_eq []))),
+    ASM_REWRITE_TAC [g_umj_monad_exp], 
+    (FIRST_ASSUM (ASSUME_TAC o MATCH_MP KdcmonadDK)),
+    REPEAT CONJ_TAC]
+  THENL (farwmmp dlD2 :: map EVERY 
+    [ ktacs2, ktacs3, ktacs4, ktacs5, ktacs6, ktacs7]) ) ;
+
+val g_umj_imp_Kmonad' = ufd (fst o EQ_IMP_RULE) g_umj_iff_Kmonad ;
+val g_umj_imp_Kmonad = 
+  fix_abs_eq [EXT_def, GSYM AND_IMP_INTRO] g_umj_imp_Kmonad' ; 
+
+val BWD_cmK = store_thm ("BWD_cmK", tmBWD_cmK, 
+  EVERY [ REPEAT STRIP_TAC,
+    (USE_LIM_RES_TAC ASSUME_TAC BWD_cm),
+    (USE_LIM_RES_TAC ASSUME_TAC (Kdc_cmonadD RSN (2, Kcmonad_IMP_Kcat))),
+    (USE_LIM_RES_TAC MATCH_MP_TAC g_umj_imp_Kmonad),
+    (ASM_REWRITE_TAC []), (CONV_TAC (fix_abs_eq_conv [])),
+    REPEAT STRIP_TAC, REFL_TAC ]) ;
 
 (*
 show_types := true ;
@@ -67,7 +444,7 @@ val (sgs, goal) = top_goal () ;
 
 val _ = set_trace "types" 1;
 val _ = set_trace "kinds" 0;
-val _ = html_theory "dist_monads";
+  val _ = html_theory "dist_monads";
 
 val _ = export_theory();
 
